Finish DTMoP!  Yayyy!

src/Parsers/DependentlyTypedMinimalOfParse.v
@@ -2,7 +2,7 @@
 Require Import Coq.Lists.List Coq.Program.Program Coq.Program.Wf Coq.Arith.Wf_nat Coq.Arith.Compare_dec Coq.Classes.RelationClasses Coq.Strings.String.
 Require Import Parsers.ContextFreeGrammar Parsers.Specification Parsers.DependentlyTyped Parsers.MinimalParse.
 Require Import Parsers.WellFoundedParse Parsers.ContextFreeGrammarProperties.
-Require Import Common Common.ilist Common.Wf.
+Require Import Common Common.ilist Common.Wf Common.Le.
 
 Set Implicit Arguments.
 
@@ -26,10 +26,9 @@ Section recursive_descent_parser.
   Variable orig_methods : @parser_computational_dataT' CharType String premethods.
   Variable gen_state : forall str0 valid (prod : production CharType) s, split_stateT str0 valid prod s.
 
-  Let P (str0 : String) valid : String -> string -> Prop
+  Definition P (str0 : String) valid : String -> string -> Prop
     := fun str p =>
-         str ≤s str0
-         /\ sub_names_listT is_valid_nonterminal_name valid initial_nonterminal_names_data
+         sub_names_listT is_valid_nonterminal_name valid initial_nonterminal_names_data
          /\ is_valid_nonterminal_name
               (if lt_dec (Length str) (Length str0)
                then initial_nonterminal_names_data
@@ -41,8 +40,8 @@ Section recursive_descent_parser.
         (H : P str0 valid str name')
   : P str0 (remove_nonterminal_name valid name) str name'.
   Proof.
-    destruct H as [ ? [ ? ? ] ].
-    split; [ assumption | split ].
+    destruct_head_hnf and.
+    repeat split; try assumption.
     { apply sub_names_listT_remove_2; assumption. }
     { destruct lt_dec; try assumption.
       match goal with
@@ -53,22 +52,22 @@ Section recursive_descent_parser.
       destruct H'; congruence. }
   Qed.
 
-  Let p_parse_item str0 valid s it
+  Definition p_parse_item str0 valid s it
     := { p' : parse_of_item String G s it & Forall_parse_of_item (P str0 valid) p' }.
-  Let p_parse_production str0 valid s p
+  Definition p_parse_production str0 valid s p
     := { p' : parse_of_production String G s p & Forall_parse_of_production (P str0 valid) p' }.
-  Let p_parse str0 valid s prods
+  Definition p_parse str0 valid s prods
     := { p' : parse_of String G s prods & Forall_parse_of (P str0 valid) p' }.
-  Let p_parse_nonterminal_name str0 valid s nonterminal_name
+  Definition p_parse_nonterminal_name str0 valid s nonterminal_name
     := { p' : parse_of_item String G  s (NonTerminal _ nonterminal_name) & Forall_parse_of_item (P str0 valid) p' }.
 
-  Let mp_parse_item str0 valid str it
+  Definition mp_parse_item str0 valid str it
     := (*{ p' :*) minimal_parse_of_item String G initial_nonterminal_names_data is_valid_nonterminal_name remove_nonterminal_name str0 valid str it(* & Forall_parse_of_item P (parse_of_item__of__minimal_parse_of_item p') }*).
-  Let mp_parse_production str0 valid str prod
+  Definition mp_parse_production str0 valid str prod
     := (*{ p' : *)minimal_parse_of_production String G initial_nonterminal_names_data is_valid_nonterminal_name remove_nonterminal_name str0 valid str prod(* & Forall_parse_of_production P (parse_of_production__of__minimal_parse_of_production p') }*).
-  Let mp_parse str0 valid str prods
+  Definition mp_parse str0 valid str prods
     := (*{ p' : *)minimal_parse_of String G initial_nonterminal_names_data is_valid_nonterminal_name remove_nonterminal_name str0 valid str prods(* & Forall_parse_of P (parse_of__of__minimal_parse_of p') }*).
-  Let mp_parse_nonterminal_name str0 valid str nonterminal_name
+  Definition mp_parse_nonterminal_name str0 valid str nonterminal_name
     := (*{ p' : *)minimal_parse_of_name String G initial_nonterminal_names_data is_valid_nonterminal_name remove_nonterminal_name str0 valid str nonterminal_name(* & Forall_parse_of_item P (parse_of_item_name__of__minimal_parse_of_name p') }*).
 
   Definition split_parse_of_production {str0 valid str it its}
@@ -166,44 +165,27 @@ Section recursive_descent_parser.
               | ParseTerminal _ => I
               | ParseNonTerminal _ _ p' => fun pf' H' => (fst H', existT _ p' (expand_forall_parse_of _ _ (snd H')))
             end pf (projT2 p)).
-    clear -pf'; subst P; simpl;
+    clear -pf'; unfold P in *; simpl;
     abstract (intros ??; do 2 edestruct lt_dec; intuition).
   Defined.
-
-Definition parse_of__of__parse_of_item' {str0 valid str nonterminal_name}
-           (p : p_parse_nonterminal_name str0 valid str nonterminal_name)
-  : P str0 valid str nonterminal_name * p_parse str0 valid str (Lookup G nonterminal_name).
-  Proof.
-    refine (match projT1 p as p' in parse_of_item _ _ str' it'
-                  return match it' with
-                           | Terminal _ => True
-                           | NonTerminal nonterminal_name' => Forall_parse_of_item (P str0 valid) p' -> P str0 valid str' nonterminal_name' * p_parse str0 valid str' (Lookup G nonterminal_name')
-                         end
-            with
-              | ParseTerminal _ => I
-              | ParseNonTerminal _ _ p' => fun H' => (fst H', existT _ p' (snd H'))
-            end (projT2 p)).
-  Defined.
-  Definition parse_of__of__parse_of_item {str0 valid str nonterminal_name} p
-    := snd (@parse_of__of__parse_of_item' str0 valid str nonterminal_name p).
   Definition parse_of__of__parse_of_item_lt {str0 valid str nonterminal_name} pf p
     := snd (@parse_of__of__parse_of_item_lt' str0 valid str nonterminal_name pf p).
 
-  Let deloop_right str0 valid str nonterminal_name
+  Definition deloop_right str0 valid str nonterminal_name
     := p_parse str0 (remove_nonterminal_name valid nonterminal_name) str (Lookup G nonterminal_name).
 
-  Let deloop_onceT
+  Definition deloop_onceT
     := forall str0 valid str nonterminal_name prods
               (p : parse_of String G str prods)
-              (pf : ~Length str < Length str0)
+              (pf : str = str0 :> String)
               (H : Forall_parse_of (P str0 valid) p),
          p_parse str0 (remove_nonterminal_name valid nonterminal_name) str prods
          + deloop_right str0 valid str nonterminal_name.
 
-  Let deloop_once_productionT
+  Definition deloop_once_productionT
     := forall str0 valid str nonterminal_name prod
               (p : parse_of_production String G str prod)
-              (pf : ~Length str < Length str0)
+              (pf : str = str0 :> String)
               (H : Forall_parse_of_production (P str0 valid) p),
          p_parse_production str0 (remove_nonterminal_name valid nonterminal_name) str prod
          + deloop_right str0 valid str nonterminal_name.
@@ -213,33 +195,25 @@ Definition parse_of__of__parse_of_item' {str0 valid str nonterminal_name}
              {str0 valid str nonterminal_name}
              {it}
              (p : parse_of_item String G str it)
-             (pf : ~Length str < Length str0)
+             (pf : str = str0 :> String)
              (H : Forall_parse_of_item (P str0 valid) p)
   : p_parse_item str0 (remove_nonterminal_name valid nonterminal_name) str it
     + deloop_right str0 valid str nonterminal_name.
   Proof.
-    refine (match p in parse_of_item _ _ str' it'
-                  return ~Length str' < Length str0
-                         -> Forall_parse_of_item (P str0 valid) p
-                         -> p_parse_item str0 (remove_nonterminal_name valid nonterminal_name) str' it'
-                            + deloop_right str0 valid str' nonterminal_name
-            with
-              | ParseTerminal _ => fun _ _ => inl (existT _ (ParseTerminal _ _ _) tt)
-              | ParseNonTerminal nonterminal_name' str'' p' =>
-                fun pf' H' =>
-                  if string_dec nonterminal_name nonterminal_name'
-                  then inr match @deloop_once _ _ _ nonterminal_name' _ p' pf' (snd H') with
-                             | inl p''' => _
-                             | inr ret => _
-                           end
-                  else match @deloop_once _ _ _ nonterminal_name _ p' pf' (snd H') with
-                         | inl p''' => inl (existT _ (ParseNonTerminal _ (projT1 p''')) (P_remove_impl _ (fst H'), projT2 p'''))
-                         | inr ret => inr ret
+    destruct p as [ | nonterminal_name' str'' p' ].
+    { exact (inl (existT _ (ParseTerminal _ _ _) tt)). }
+    { refine (if string_dec nonterminal_name nonterminal_name'
+              then inr match @deloop_once _ _ _ nonterminal_name' _ p' pf (snd H) with
+                         | inl p''' => _
+                         | inr ret => _
                        end
-            end pf H);
-    clear deloop_once;
-    solve [ assumption
-          | subst; assumption ].
+              else match @deloop_once _ _ _ nonterminal_name _ p' pf (snd H) with
+                     | inl p''' => inl (existT _ (ParseNonTerminal _ (projT1 p''')) (P_remove_impl _ (fst H), projT2 p'''))
+                     | inr ret => inr ret
+                   end);
+      clear deloop_once;
+      solve [ assumption
+            | subst; assumption ]. }
   Defined.
 
   Definition deloop_once'
@@ -259,6 +233,36 @@ Definition parse_of__of__parse_of_item' {str0 valid str nonterminal_name}
              end. }
   Defined.
 
+  Local Ltac deloop_t :=
+    repeat match goal with
+             | _ => assumption
+             | _ => intro
+             | [ H : ?x = ?y |- _ ] => subst x
+             | [ H : ?x = ?y |- _ ] => subst y
+             | [ H : _ ≤s _ |- _ ] => destruct H
+             | _ => progress simpl in *
+             | [ H : _ |- _ ] => rewrite Length_Empty in H
+             | _ => rewrite Length_Empty
+             | [ H : _ < 0 |- _ ] => destruct (Lt.lt_n_0 _ H)
+             | _ => progress destruct_head and
+             | [ |- _ /\ _ ] => split
+             | [ H : sub_names_listT _ _ _ |- is_valid_nonterminal_name _ _ = true ]
+               => (apply H; eapply sub_names_listT_remove; eassumption)
+             | [ H : ~0 < ?n |- _ ]
+               => (let H' := fresh in
+                   destruct (zerop n) as [ | H' ]; [ clear H | destruct (H H') ])
+             | [ H : Length _ = 0 |- _ ] => apply Empty_Length in H
+             | [ H : ?x <> ?x |- _ ] => destruct (H eq_refl)
+             | [ H : context[Length (_ ++ _)] |- _ ] => rewrite <- Length_correct in H
+             | [ H : ~_ < _ + _ |- _ ]
+               => unique pose proof (proj1 (not_lt_plus H))
+             | [ H : ~_ < _ + _ |- _ ]
+               => unique pose proof (proj2 (not_lt_plus H))
+             | [ H : ?T, H' : ~?T |- _ ] => destruct (H' H)
+             | [ H : ~ ?a < ?a + _ |- _ ] => apply not_lt_add_r in H
+             | [ H : ~ ?a < _ + ?a |- _ ] => apply not_lt_add_l in H
+           end.
+
   Definition deloop_once_production'
              (deloop_once : deloop_onceT)
              (deloop_once_production : deloop_once_productionT)
@@ -269,17 +273,17 @@ Definition parse_of__of__parse_of_item' {str0 valid str nonterminal_name}
     { refine (inl (existT _ (ParseProductionNil _ _) tt)). }
     { (** We must discriminate based on whether or not [str] has already gotten shorter *)
       destruct (stringlike_dec str' (Empty _)) as [e|e], (stringlike_dec strs' (Empty _)) as [e'|e'];
-      try (assert (pf0 : ~Length str' < Length str0)
+      try (assert (pf0 : str' = str0)
             by (clear -pf e'; abstract (subst strs'; rewrite ?RightId, ?LeftId in pf; exact pf));
            pose proof (@deloop_once_item' (deloop_once) str0 valid _ nonterminal_name pat' p' pf0 (fst H)) as deloop_once_item;
            clear deloop_once);
-      try (assert (pf1 : ~Length strs' < Length str0)
+      try (assert (pf1 : strs' = str0)
             by (clear -pf e; abstract (subst str'; rewrite ?RightId, ?LeftId in pf; exact pf));
            specialize (deloop_once_production str0 valid _ nonterminal_name pats' p'' pf1 (snd H)));
       try (destruct deloop_once_item as [ret|ret];
-           [ | right; subst; rewrite ?LeftId, ?RightId; assumption ]);
+           [ | right; repeat first [ subst str' | subst strs' ]; rewrite ?LeftId, ?RightId; assumption ]);
       try (destruct deloop_once_production as [ret'|ret'];
-           [ | right; subst; rewrite ?LeftId, ?RightId; assumption ]).
+           [ | right; repeat first [ subst str' | subst strs' ]; rewrite ?LeftId, ?RightId; assumption ]).
       { (** empty, empty *)
         left.
         exists (ParseProductionCons (projT1 ret) (projT1 ret')).
@@ -288,141 +292,52 @@ Definition parse_of__of__parse_of_item' {str0 valid str nonterminal_name}
         left.
         exists (ParseProductionCons p' (projT1 ret')).
         refine (expand_forall_parse_of_item _ (fst H), projT2 ret').
-        admit. }
-      admit.
-      admit. }
-  Defined.
-  (*
-        clear -e e'.
-        hnf.
-        pose proof (@deloop_once_item' (deloop_once) str' valid _ nonterminal_name pat' p' pf0 (fst H)) as deloop_once_item;
-           clear deloop_once
-
-
-
-        constructor (assumption).
-        Focus 2.
-        specialize (fun pf X
-        simpl in H.
-
-      specialize (fun h' pf
-                        => @minimal_parse_of_name__of__parse_of_name
-                             h' (transitivity pf (Lt.lt_n_Sn _))).
-            change (S ((size_of_parse_item p0')
-                       + (size_of_parse_production p1'))
-                    < S h') in H_h.
-            apply Lt.lt_S_n in H_h.
-            pose proof (Lt.le_lt_trans _ _ _ (Plus.le_plus_l _ _) H_h) as H_h0.
-            pose proof (Lt.le_lt_trans _ _ _ (Plus.le_plus_r _ _) H_h) as H_h1.
-            clear H_h.
-            pose proof (fun valid Hinit => @minimal_parse_of_item__of__parse_of_item _ h'  minimal_parse_of_name__of__parse_of_name _ (transitivity (str_le1_append _ _ _) pf) valid _ p0' H_h0 Hinit (fst H_forall)) as p_it.
-            pose proof (fun valid Hinit => @minimal_parse_of_production__of__parse_of_production h' minimal_parse_of_name__of__parse_of_name _ (transitivity (str_le2_append _ _ _) pf) valid _ p1' H_h1 Hinit (snd H_forall)) as p_prod.
-            destruct (stringlike_dec str' (Empty _)), (stringlike_dec str'' (Empty _));
-              subst.
-            { (* empty, empty *)
-              specialize (p_it valid' Hinit'); specialize (p_prod valid' Hinit').
-              destruct p_it as [ [ p0'' H0''] |], p_prod as [ [ p1'' H1'' ] |];
-                [ | | | ];
-                min_parse_prod_t. }
-            { (* empty, nonempty *)
-              specialize (p_it initial_names_data (reflexivity _)); specialize (p_prod valid' Hinit').
-              destruct p_it as [ [ p0'' H0''] |], p_prod as [ [ p1'' H1'' ] |];
-                [ | | | ];
-                min_parse_prod_t;
-                min_parse_prod_pose_t;
-                min_parse_prod_t. }
-            { (* nonempty, empty *)
-              specialize (p_it valid' Hinit'); specialize (p_prod initial_names_data (reflexivity _)).
-              destruct p_it as [ [ p0'' H0''] |], p_prod as [ [ p1'' H1'' ] |];
-                [ | | | ];
-                min_parse_prod_t;
-                min_parse_prod_pose_t;
-                min_parse_prod_t. }
-            { (* nonempty, nonempty *)
-              specialize (p_it initial_names_data (reflexivity _)); specialize (p_prod initial_names_data (reflexivity _)).
-              destruct p_it as [ [ p0'' H0''] |], p_prod as [ [ p1'' H1'' ] |];
-                [ | | | ];
-                min_parse_prod_t;
-                min_parse_prod_pose_t;
-                min_parse_prod_t. } }
-
-refine (match
-                 deloop_once_item' (@deloop_once) p' pf H,
-                 deloop_once_production p'' pf H
-               with
-                 | _, _ => _
-               end).
-
-    { refine match deloop_once_production str0 valid str' nonterminal_name _ p' pf H with
-               | inl ret => inl (existT _ (ParseHead pats' (projT1 ret)) (projT2 ret))
-               | inr ret => inr ret
-             end. }
-    { refine match deloop_once str0 valid str' nonterminal_name _ p' pf H with
-               | inl ret => inl (existT _ (ParseTail _ (projT1 ret)) (projT2 ret))
-               | inr ret => inr ret
-             end. }
+        unfold P in *; simpl.
+        clear -e e' pf1 remove_nonterminal_name_1 remove_nonterminal_name_2.
+        abstract (intros; edestruct lt_dec; deloop_t). }
+      { (** nonempty, empty *)
+        left.
+        exists (ParseProductionCons (projT1 ret) p'').
+        refine (projT2 ret, expand_forall_parse_of_production _ _ (snd H)).
+        unfold P in *; simpl.
+        clear -e e' pf0 remove_nonterminal_name_1 remove_nonterminal_name_2.
+        abstract (intros; edestruct lt_dec; deloop_t). }
+      { (** nonempty, nonempty *)
+        left.
+        exists (ParseProductionCons p' p'').
+        refine (expand_forall_parse_of_item _ (fst H),
+                expand_forall_parse_of_production _ _ (snd H));
+          unfold P in *; simpl;
+          clear -e e' pf remove_nonterminal_name_1 remove_nonterminal_name_2;
+          abstract (intros; edestruct lt_dec; deloop_t). } }
   Defined.
 
+  Fixpoint deloop_once {str0 valid str nonterminal_name pats} (p : parse_of String G str pats)
+    := @deloop_once' (@deloop_once) (@deloop_once_production) str0 valid str nonterminal_name pats p
+  with deloop_once_production {str0 valid str nonterminal_name pat} (p : parse_of_production String G str pat)
+       := @deloop_once_production' (@deloop_once) (@deloop_once_production) str0 valid str nonterminal_name pat p.
+  Definition deloop_once_item {str0 valid str nonterminal_name it} (p : parse_of_item String G str it)
+    := @deloop_once_item' (@deloop_once) str0 valid str nonterminal_name it p.
 
-
-  Fixpoint deloop_once
-  {str0 valid str nonterminal_name}
-           {pats}
-           (p : parse_of String G str pats)
-    := match p in parse_of _ _ str' pats'
-             return ~Length str' < Length str0
-                    -> Forall_parse_of (P str0 valid) p
-                    -> p_parse str0 (remove_nonterminal_name valid nonterminal_name) str' pats'
-                       + p_parse str0 (remove_nonterminal_name valid nonterminal_name) str' (Lookup G nonterminal_name)
-       with
-         | ParseHead str' pat' pats' p'
-           => fun pf H
-              => match deloop_once_production p' pf H with
-                   | inl ret => inl (existT _ (ParseHead pats' (projT1 ret)) ((projT2 ret) : Forall_parse_of (P str0 (remove_nonterminal_name valid nonterminal_name)) (ParseHead _ (projT1 ret))))
-                   | inr ret => inr ret
-                 end
-         | ParseTail _ _ _ p'
-           => fun pf H
-              => match deloop_once p' pf H with
-                   | inl ret => inl (existT _ (ParseTail (projT1 ret)) (projT2 ret))
-                   | inr ret => inr ret
-                 end
-       end
-  with deloop_once_production
-         {str0 valid str nonterminal_name}
-         {pat}
-         (p : parse_of_production String G str pat)
-       := match p in parse_of_production _ _ str' pat'
-                return ~Length str' < Length str0
-                       -> Forall_parse_of_production (P str0 valid) p
-                       -> p_parse_production str0 (remove_nonterminal_name valid nonterminal_name) str' pat'
-                          + p_parse str0 (remove_nonterminal_name valid nonterminal_name) str' (Lookup G nonterminal_name)
-          with
-            | ParseProductionNil => fun _ _ => inl (existT _ ParseProductionNil tt)
-            | ParseProductionCons str pat strs pats p' p''
-              => fun pf H
-                 => match
-                     deloop_once_item' (@deloop_once) p' pf H,
-                     deloop_once_production p'' pf H
-                   with
-                     | _ => admit
-                   end
-          end.
-    with expand_forall_parse_of_production {str pat} {p : parse_of_production String G str pat}
-         : Forall_parse_of_production P p -> Forall_parse_of_production P' p
-         := match p return Forall_parse_of_production P p -> Forall_parse_of_production P' p with
-              | ParseProductionNil => fun x => x
-              | ParseProductionCons str pat strs pats p' p''
-                => fun ab => (expand_forall_parse_of_item' (@expand_forall_parse_of) (fst ab),
-                              expand_forall_parse_of_production (snd ab))
-            end.
-
-    Global Arguments expand_forall_parse_of : simpl never.
-    Global Arguments expand_forall_parse_of_production : simpl never.
-
-    Definition expand_forall_parse_of_item {str it} {p : parse_of_item String G str it}
-      := @expand_forall_parse_of_item' _ (@expand_forall_parse_of) str it p.
-*)
+  Definition parse_of__of__parse_of_item_eq' {str0 valid str nonterminal_name}
+             (pf : str = str0 :> String)
+             (p : p_parse_nonterminal_name str0 valid str nonterminal_name)
+  : P str0 valid str nonterminal_name * p_parse str0 (remove_nonterminal_name valid nonterminal_name) str (Lookup G nonterminal_name).
+  Proof.
+    refine (match projT1 p as p' in parse_of_item _ _ str' it'
+                  return match it' with
+                           | Terminal _ => True
+                           | NonTerminal nonterminal_name' => str' = str0 -> Forall_parse_of_item (P str0 valid) p' -> P str0 valid str' nonterminal_name' * p_parse str0 (remove_nonterminal_name valid nonterminal_name') str' (Lookup G nonterminal_name')
+                         end
+            with
+              | ParseTerminal _ => I
+              | ParseNonTerminal nonterminal_name' _ p'
+                => fun pf' H' => (fst H', if @deloop_once str0 valid _ nonterminal_name' _ p' pf' (snd H') then _ else _)
+            end pf (projT2 p));
+    assumption.
+  Defined.
+  Definition parse_of__of__parse_of_item_eq {str0 valid str nonterminal_name} pf p
+    := snd (@parse_of__of__parse_of_item_eq' str0 valid str nonterminal_name pf p).
 
   Local Instance strdata : @parser_computational_strdataT _ String G _ _
     := {| lower_nonterminal_name_state str0 valid nonterminal_name str st := st;
@@ -443,9 +358,7 @@ refine (match
                            end (projT2 p)
              end;
           lift_lookup_nonterminal_name_state_lt str0 valid nonterminal_name str pf := option_map (parse_of__of__parse_of_item_lt pf);
-          lift_lookup_nonterminal_name_state_eq1 str0 valid nonterminal_name str pf := option_map _(*parse_of__of__parse_of_item*) |}.
-
-
+          lift_lookup_nonterminal_name_state_eq str0 valid nonterminal_name str pf := option_map (parse_of__of__parse_of_item_eq pf) |}.
 
   Section minimal.
     Local Ltac t' :=
@@ -469,10 +382,6 @@ refine (match
       end.
 
     Section parts.
-      Let alt_option valid str
-        := { nonterminal_name : _ & (is_valid_nonterminal_name valid nonterminal_name = false /\ P nonterminal_name)
-                                    * p_parse str (Lookup G nonterminal_name) }%type.
-
       Section common.
         Section types.
           Context (str0 : String)
@@ -488,7 +397,7 @@ refine (match
                        /\ is_valid_nonterminal_name valid nonterminal_name = false }*).
 
           Section T_nonterminal_name.
-            Context (name : string) (str : StringWithSplitState String (split_stateT (include_nonterminal_name _ name))).
+            Context (name : string) (str : StringWithSplitState String (split_stateT str0 valid (include_nonterminal_name _ name))).
             Let ret := mp_parse_nonterminal_name str0 valid str name.
 
             Definition T_nonterminal_name_success  : Type
@@ -502,7 +411,7 @@ refine (match
           End T_nonterminal_name.
 
           Section T_item.
-            Context (it : item CharType) (str : StringWithSplitState String (split_stateT it)).
+            Context (it : item CharType) (str : StringWithSplitState String (split_stateT str0 valid it)).
 
             Let ret := mp_parse_item str0 valid str it.
 
@@ -516,7 +425,7 @@ refine (match
           End T_item.
 
           Section T_production.
-            Context (prod : production CharType) (str : StringWithSplitState String (split_stateT prod)).
+            Context (prod : production CharType) (str : StringWithSplitState String (split_stateT str0 valid prod)).
 
             Let ret := mp_parse_production str0 valid str prod.
 
@@ -530,7 +439,7 @@ refine (match
           End T_production.
 
           Section T_productions.
-            Context (prods : productions CharType) (str : StringWithSplitState String (split_stateT prods)).
+            Context (prods : productions CharType) (str : StringWithSplitState String (split_stateT str0 valid prods)).
 
             Let ret := mp_parse str0 valid str prods.
 
@@ -556,96 +465,6 @@ refine (match
                 T_production_failure := T_production_failure;
                 T_productions_success := T_productions_success;
                 T_productions_failure := T_productions_failure |}.
-
-
-        Definition split_list_completeT
-                   (str0 : String)
-                   valid1 valid2
-                   (it : item CharType) (its : production CharType)
-                   (str : StringWithSplitState String (split_stateT (it::its : production CharType)))
-                   (pf : str ≤s str0)
-                   (split_list : list (StringWithSplitState String (split_stateT it) * StringWithSplitState String (split_stateT its)))
-          := ({ s1s2 : String * String
-                       & (fst s1s2 ++ snd s1s2 =s str)
-                         * (minimal_parse_of_item _ G initial_nonterminal_names_data is_valid_nonterminal_name remove_nonterminal_name str0 valid1 (fst s1s2) it)
-                         * (minimal_parse_of_production _ G initial_nonterminal_names_data is_valid_nonterminal_name remove_nonterminal_name str0 valid2 (snd s1s2) its) }%type)
-             -> ({ s1s2 : _
-                          & (In s1s2 split_list)
-                            * (minimal_parse_of_item _ G initial_nonterminal_names_data is_valid_nonterminal_name remove_nonterminal_name str0 valid1 (fst s1s2) it)
-                            * (minimal_parse_of_production _ G initial_nonterminal_names_data is_valid_nonterminal_name remove_nonterminal_name str0 valid2 (snd s1s2) its) }%type).
-
-        (*Lemma H_prod_split'_helper
-              (str0 : String)
-              (valid : nonterminal_names_listT)
-              (it : item CharType) (its : production CharType)
-              (str : StringWithSplitState String (split_stateT it))
-              (strs : StringWithSplitState String (split_stateT its))
-              (p_it : minimal_parse_of_item String G initial_nonterminal_names_data is_valid_nonterminal_name remove_nonterminal_name str0 valid str it)
-              (p_its : minimal_parse_of_production String G initial_nonterminal_names_data is_valid_nonterminal_name remove_nonterminal_name str0 valid strs its)
-              (ls : list
-                      (StringWithSplitState String (split_stateT it) *
-                       StringWithSplitState String (split_stateT its)))
-              (Hin : In (str, strs) ls)
-              (H : fold_right
-                     Datatypes.prod
-                     unit
-                     (map
-                        (fun s1s2 =>
-                           let s1 := fst s1s2 in
-                           let s2 := snd s1s2 in
-                           ((@T_item_failure str0 valid it s1 * @T_production_failure str0 valid its s2)
-                            + (@T_item_success str0 valid it s1 * @T_production_failure str0 valid its s2)
-                            + (@T_item_failure str0 valid it s1 * @T_production_success str0 valid its s2))%type)
-                        ls))
-        : False.
-        Proof.
-          induction ls; simpl in *; trivial; [].
-          destruct_head or; subst;
-          destruct_head prod; eauto; [].
-          destruct_head sum; destruct_head prod;
-          unfold T_item_failure, T_item_success, T_production_failure, T_production_success in *;
-          eauto.
-        Qed.
-
-        Definition H_prod_split'
-                   (str0 : String)
-                   (valid : nonterminal_names_listT)
-                   it its
-                   (str : StringWithSplitState String (split_stateT (it::its : production CharType)))
-                   pf
-                   (split_list_complete : @split_list_completeT str0 valid valid it its str pf (split_string_for_production it its str))
-        : @split_string_lift_T _ String _ str0 valid it its str (split_string_for_production it its str).
-        Proof.
-          clear -split_list_complete.
-          intros H pf' H'; hnf in H', split_list_complete.
-          destruct str as [str st]; simpl in *.
-          inversion H'; clear H'; subst.
-          specialize (fun s1 s2 b
-                      => split_list_complete
-                           (existT _ (s1, s2) b));
-            simpl in *.
-          let p_it := hyp_with_head @minimal_parse_of_item in
-          let p_its := hyp_with_head @minimal_parse_of_production in
-          specialize (fun pf => split_list_complete _ _ (pf, p_it, p_its)).
-          repeat match goal with
-                   | [ H : ?T -> ?A |- _ ]
-                     => let H' := fresh in
-                        assert (H' : T) by (apply bool_eq_correct; reflexivity);
-                          specialize (H H'); clear H'
-                   | _ => progress destruct_sig
-                   | _ => progress destruct_head option
-                   | _ => progress destruct_head or
-                   | _ => progress destruct_head False
-                   | _ => progress subst
-                   | [ H : (_, _) = (_, _) |- _ ] => inversion H; clear H
-                 end.
-          { eapply H_prod_split'_helper; try eassumption;
-            try match goal with H : _ |- _ => exact H end;
-            try instantiate (1 := [(_, _)]);
-            [ left; reflexivity | split; assumption ]. }
-          { eapply H_prod_split'_helper; try eassumption;
-            try match goal with H : _ |- _ => exact H end. }
-        Qed.*)
 
         Hint Constructors minimal_parse_of minimal_parse_of_name minimal_parse_of_production minimal_parse_of_item unit prod unit : minimal_instance_db.
         Hint Unfold T_item_success T_item_failure T_production_success T_production_failure T_productions_success T_productions_failure T_nonterminal_name_success T_nonterminal_name_failure
@@ -739,6 +558,7 @@ refine (match
             | [ H : (_, _) = (_, _) |- _ ] => apply path_prod' in H
             | [ H : ?T |- _ ] => match eval hnf in T with
                                    | (_ * _)%type => destruct H
+                                   | (_ /\ _)%type => destruct H
                                  end
             | _ => progress subst
             | _ => progress simpl
@@ -765,16 +585,12 @@ Please report." *)
             | [ H : minimal_parse_of_item _ _ _ _ _ _ _ _ (Terminal _) |- _ ] => (* work around 4035 *) let H' := fresh in rename H into H'; dependent destruction H'
             | [ H : minimal_parse_of _ _ _ _ _ _ _ _ (_::_) |- _ ] => (* work around 4035 *) let H' := fresh in rename H into H'; dependent destruction H'
             | [ H : parse_of _ _ _ (_::_) |- _ ] => (* work around 4035 *) let H' := fresh in rename H into H'; dependent destruction H'
+            | [ H : appcontext[if lt_dec ?a ?b then _ else _] |- _ ]
+              => destruct (lt_dec a b)
           end.
-
-        (*Local Ltac should_
-        Local Ltac pre_congruence_avoid_anomalies
-          := repeat match goal with
-                      | [ H : ?T |- _ ]*)
 
         Local Ltac t' :=
           first [ t''
-                (*| congruence*)
                 | match goal with H : true = false |- _ => exfalso; clear -H; congruence end
                 | match goal with H : ?x = false, H' : ?x = true |- _ => exfalso; clear -H H'; abstract congruence end
                 | abstract omega
@@ -802,16 +618,16 @@ Please report." *)
         Lemma cons_success
               (str0 : String) (valid : nonterminal_names_listT)
               (it : item CharType) (its : production CharType)
-              (s1 : StringWithSplitState String (split_stateT it))
-              (s2 : StringWithSplitState String (split_stateT its))
-              (str : StringWithSplitState String (split_stateT (it :: its : production CharType)))
+              (s1 : StringWithSplitState String (split_stateT str0 valid it))
+              (s2 : StringWithSplitState String (split_stateT str0 valid its))
+              (str : StringWithSplitState String (split_stateT str0 valid (it :: its : production CharType)))
         : let a1 := DependentlyTyped.T_item_success str0 valid it s1 in
           let a2 := DependentlyTyped.T_production_success str0 valid its s2 in
           let ret :=
               DependentlyTyped.T_production_success str0 valid (it :: its) str in
           str ≤s str0 ->
           s1 ++ s2 =s str ->
-          In (s1, s2) (split_string_for_production it its str) -> a1 -> a2 -> ret.
+          In (s1, s2) (split_string_for_production str0 valid it its str) -> a1 -> a2 -> ret.
         Proof.
           destruct str as [ ? [ ] ]; simpl.
           { intros ? ? H.
@@ -832,8 +648,8 @@ Please report." *)
 
         Local Obligation Tactic := idtac.
 
-        Let H_prod_splitT' str0 valid it its str st
-          := split_string_lift_T str0 valid it its {| string_val := str ; state_val := st |} (split_string_for_production it its {| string_val := str ; state_val := st |}).
+        Definition H_prod_splitT' str0 valid it its str st
+          := split_string_lift_T str0 valid it its {| string_val := str ; state_val := st |} (split_string_for_production str0 valid it its {| string_val := str ; state_val := st |}).
 
         Lemma H_prod_split_helper str0 valid it its str st
         : @H_prod_splitT' str0 valid it its str (Some st).
@@ -851,8 +667,7 @@ Please report." *)
           { repeat t''. }
         Defined.
 
-        Start Profiling.
-        Time Global Program Instance minimal_parser_dependent_types_extra_data
+        Global Program Instance minimal_parser_dependent_types_extra_data
              (H_prod_split' : forall str0 valid it its str, @H_prod_splitT' str0 valid it its str None)
                (*(split_list_complete : forall str0 valid it its str pf, @split_list_completeT str0 valid valid it its str pf (split_string_for_production it its str))*)
         : @parser_dependent_types_extra_dataT _ String G
@@ -865,10 +680,6 @@ Please report." *)
                             | Some st => @H_prod_split_helper str0 valid it its str' st
                           end
                    end |}.
-        Obligation 12. t. Defined.
-        Obligation 13. t. Defined.
-        Obligation 14. t. Defined.
-        Obligation 11. t. Defined.
         Obligation 1. t. Defined.
         Obligation 2. t. Defined.
         Obligation 3. t. Defined.
@@ -879,861 +690,12 @@ Please report." *)
         Obligation 8. t. Defined.
         Obligation 9. t. Defined.
         Obligation 10. t. Defined.
-        Obligation 15.
-        simpl.
-        intros.
-        assert (str = str0 :> String).
-        { destruct_head @str_le.
-          { exfalso; eauto with nocore. }
-          { assumption. } }
-        subst.
-        clear H H0.
-        hnf.
-        repeat t''0; [ | solve [ t ] ].
-        clear H.
-        hnf in p.
-        destruct p.
-        dependent destruction x.
-        destruct f.
-
-        hnf in p0.
-
-
-        do 10 t''.
-        t''.
-        t''.
-        t''.
-        t''.
-        t''.
-        t''.
-        destruct_head prod.
-        destruct_head sum; repeat t''.
-        t''.
-        match goal with
-        end.
-        simpl split_string_for_production in *.
-        t''.
-        t''.
-        simpl in X.
-        destruct_head prod.
-        destruct_head sum.
-        repeat t''.
-        repeat t''.
-        repeat t''.
-simpl in *.
-        do 10 (simpl in *; t'').
-        t''.
-        t''.
-        t''.
-        t''.
-        t''.
-        t''.
-        t''; simpl in *.
-        t''; simpl in *.
-        t''; simpl in *.
-        t''; simpl in *.
-        t''; simpl in *.
-        t''; simpl in *.
-        t''; simpl in *.
-        t''; simpl in *.
-        simpl in X.
-        t''.
-        t''.
-        t''.
-        t''.
-        t''.
-        t''.
-        t''.
-        t''.
-        t''.
-        t''.
-        t''.
-        t''.
-        t''.
-
-        t''.
-        simpl in s.
-t. Defined.
-        Obligation 16. t. Defined.
-        Next Obligation. t. Defined.
-        Next Obligation. t. Defined.
-        Next Obligation. t. Defined.
-        Next Obligation. t. Defined.
-        Next Obligation. t. Defined.
-        Next Obligation. t. Defined.
-        Next Obligation. t. Defined.
-        Next Obligation. t. Defined.
-        Next Obligation. t. Defined.
-        Next Obligation. t. Defined.
-        Next Obligation. simpl.
-                        do 5 t''.
-                        do 5 t''.
-                        do 5 t''.
-                        t''.
-                        t''.
-                        t''.
-                        t''.
-                        t''.
-                        t''.
-                        t''.
-                        t''.
-                        t''.
-                        match goal with
-                        end.
-                        t''.
-                        do 5 t''.
-                        do 5 t''.
-                        do 5 t''.
-                        do 5 t''.
-                        do 5 t''.
-t. Defined.
-
-        Obligation 15.
-   (forall (str0 : String) (valid : nonterminal_names_listT)
-      (it : item CharType) (its : production CharType)
-      (str : String), H_prod_splitT' str0 valid None) ->
-   forall (str0 : String) (valid : nonterminal_names_listT)
-     (nonterminal_name : string)
-     (str : StringWithSplitState String
-              (split_stateT
-                 (include_nonterminal_name CharType nonterminal_name))),
-   let ret :=
-     DependentlyTyped.T_nonterminal_name_failure str0 valid nonterminal_name
-       str in
-   let arg :=
-     DependentlyTyped.T_productions_failure str0
-       (remove_nonterminal_name valid nonterminal_name)
-       (G nonterminal_name)
-       (lift_StringWithSplitState lift_lookup_nonterminal_name_state str) in
-   ~ Length str < Length str0 -> arg -> ret
-
-
-
-t. repeat t''.
-        apply remove_nonterminal_name_2 in H3.
-
-        exists x.
-        repeat t''.
-        destruct H3.
-        repeat t''.
-        split.
-        repeat t''.
-        repeat t''.
-        hnf in p0.
-        repeat t''.
-        hnf in p0.
-        SerachAbout
-
-
-        dependent destruction x.
-        repeat t''.
-        destruct f.
-        hnf in p0.
-        SearchAbout sub_names_listT.
-        pose (sub_names_listT_remove is_valid_nonterminal_name remove_nonterminal_name remove_name_1 _ _ _ H3).
-        SearchAbout sub_names_listT.
-        unique pose proof (
- Defined.
-        Obligation 16.
-
-        t.
-        { repeat t''.
-          dependent destruction x.
-          repeat t''.
-          destruct f.
-          repeat t''.
-          hnf in p0.
-          repeat t''.
-          hnf in H3.
-          specialize (H3 _ p0).
-          simpl in f.
-          destruct f.
-          hnf in p0.
-
- t. Defined.
-        Next Obligation. t. Defined.
-        Next Obligation. t. Defined.
-        Next Obligation. t. Defined.
-        Next Obligation. t. Defined.
-        Next Obligation. t. Defined.
-        Next Obligation. t. Defined.
-        Next Obligation. t. Defined.
-        Next Obligation. t. Defined.
-        Next Obligation. t. Defined.
-        Next Obligation. t. Defined.
-        Next Obligation. t. Defined.
-        Next Obligation. t.
-                         repeat t''.
-Set Printing All.
-            lazymatch goal with | [ H : sub_names_listT _ ?x ?y -> _ |- _ ] => specialize (H (reflexivity _)) end.
-                         specialize (X (reflexivity _)).
-                         Obligations.
- Defined.
-        Next Obligation. t. Defined.
-        Next Obligation. t. Defined.
-        Next Obligation. t. Defined.
-        Next Obligation. t. Defined.
-        Next Obligation. t. Defined.
-        Next Obligation. t. Defined.
-          Start Profiling.
-          t.
-          Show Profile.
-
-          repeat t''0.
-          simpl in *.
-          Show Profile.
-          { repeat t''.
-
-
-          repeat t''.
-
-t. Defined.
-        Next Obligation. t. Defined.
-        Next Obligation. t. Defined.
-        Next Obligation. t. Defined.
-        Next Obligation. t. Defined.
-        Next Obligation. t. Defined.
-        Next Obligation. t. Defined.
-        Next Obligation. t. Defined.
-        Next Obligation. t. Defined.
-Definition heap_is_star (H1 H2 : hprop) : hprop := ...
-Open Scope heap_scope.
-Bind Scope heap_scope with hprop.
-Delimit Scope heap_scope with h.
-Notation "P ==>+ Q" := (pred_le P (heap_is_star P Q))
-  (at level 55) : heap_scope_advanced.
-
-
-which I could (finally) solve by adding (non-intuitive) explicit scopes:
-
-Notation "P ==>+ Q" := (pred_le P%h (heap_is_star P Q))
-  (at level 55) : heap_scope_advanced.
-
- Defined.
-        Next Obligation. t. Defined.
-        Next Obligation. t. Defined.
-        Next Obligation. t. Defined.
-        Next Obligation. t. Defined.
-        Next Obligation. t. Defined.
-        Next Obligation. t. Defined.
-        Next Obligation. t. Defined.
-        Next Obligation. t. Defined.
-        Next Obligation. t. repeat t''.
-                         simpl in H.
-                         simpl in *.
-                         Focus 2.
-                         simpl in *.
-                         subst_body.
-                         simpl in *.
-                         repeat t''.
-                         dependent destruction x.
-
-                         repeat t''.
-                         simpl in *.
-                         t.
-                         apply X.
-                         exists m.
-                         t.
-                         t.
-                         simpl in *.
-                         apply X0.
-                         exists x.
-                         t.
-                         simpl in *.
-                         repeat t'.
-
-                         dependent destruction x.
-                         simpl in *.
-                         repeat t''.
-                         repeat t'.
-
-                         Obligations.
-Defined.
-        Next Obligation. t. Defined.
-        Next Obligation. t. Defined.
-        Obligations.
-        Next Obligation.
-          subst_body; simpl in *.
-
-          repeat t''.
-          subst_body.
-          repeat t''.
-          dependent destruction x; t.
-          repeat t''.
-
-          Print minimal_parse_of.
-          Focus 2.
-          lazymatch goal with
-          end.
-
-
-
-        Obligation 16. t. repeat t''.
-        subst_body. simpl in *.
- Defined. subst_body. repeat t''.
-
- Defined.
-        Next Obligation.
-repeat t''.
-
- Defined.
-        Next Obligation. t. Defined.
-        Next Obligation. t. Defined.
-
-
-        Defined.
-        Next Obligation. t. Defined.
-
-          Next Obligation
-          simpl.
- do 25 try t''.
-                         t''.
-                         t''.
-                         t''.
-                         t''.
-                         t''.
-                         t''.
-                         t''.
-                         t''.
-                         t''.
-                         t''.
-                         t''.
-                         t''.
-                         t''.
-                         t''.
-                         t''.
-                         t''.
-                         t''.
-                         subst_body.
-                         simpl in *.
-                         t''.
-                         t''.
-                         t''.
-                         t''.
-                         t''.
-                         t''.
-                         t''.
-                         t''.
-                         Show Profile.
-                         t''.
-
-      (s1 s2 : StringWithSplitState A (fun x => option (P x)))
-:
-                         match goal with
-                           | [ H : {| state_val := Some _ |} = {| state_val := None |} |- _ ]
-                             => exfalso; clear -H
-                         end.
-                         apply (f_equal_dep (@state_val _ _)) in H0.
-                         refine (_, f0).
-                         exact f.
-                         match goal with
-            | [ b : Forall_parse_of_production _ _ |- Forall_parse_of_production _ _ ]
-              => refine (_, b)
-end.
-                         t''.
-
-                         lazymatch goal with
-                         | [ x : minimal_parse_of_item _ _ _ _ _ _ _ _ _, y : minimal_parse_of_production _ _ _ _ _ _ _ _ _, H : _ \/ _ |- _ ] => idtac end.
-                         match goal with [ |- @sigT ?A _ ]
-                           => idtac
-                         end.
-
-exists (MinParseProductionCons H x y : A)
-
-t000.
-Show Profile.
-                         :
-                         SearchAbout ((_, _) = (_, _)).
-                         t''.
-                         t''.
-                         t''.
-                         t''.
-                         t''.
-                         t''.
-                         do 10 try t''.
-                         t''.
-                         let H := match goal with H : _ \/ False |- _ => constr:H end.
-
-                         t''.
-                         Show Profile.
-          simpl.
-        Obligation 8. t. Defined.
-        Obligation 9. t. Defined.
-        Obligation 10. t. Defined.
-        Obligation 8. t. Defined.
-        Obligations.
-        repeat t''.
-        inversion x.
- Defined.
-        Obligations.
-        Next Obligation. Show Profile.
-                         repeat t''.
-
-                         Time match goal with
-
-                         end.
-
-                         exact (f2, f0).
-                         t''.
-                         t''.
-                         t''.
-                         t''.
-                         t''.
-                         t''.
-                         t''.
-                         t''.
-                         t''.
-                         t''.
-                         t''.
-                         t''.
-                         t''.
-                         t''.
-                         t''.
-                         t''.
-                         t''.
-                         t''.
-                         t''.
-                         t''.
-                         t''.
-                         t''.
-                         t''.
-                         t''.
-                         t''.
-                         t''.
-                         t''.
-                         t''.
-                         t''.
-                         t''.
-                         t''.
-                         t''.
-                         t''.
-                         subst_body.
-                         t''.
-                         t''.
-                         t''.
-                         t''.
-                         t''.
-
-                         repeat t''.
-                         subst_body.
-                         progress t''.
-                         progress t''.
-                         progress t''.
-                         progress t''.
-                         dest
-                         progress t''.
-                         progress t''.
-                         progress t''.
-                         progress t''.
-                         progress t''.
-                         progress t''.
-                         progress t''.
-                         progress t''.
-                         progress t''.
-                         progress t''.
-                         progress t''.
-                         progress t''.
-                         progress t''.
-                         progress t''.
-                         progress t''.
-                         progress t''.
-                         progress t''.
-                         progress t''.
-                         progress t''.
-                         progress t''.
-                         progress t''.
-                         progress t''.
-                         progress t''.
-Time match goal with
-                           .
-Show
-
- Defined.
-        Next Obligation. t. Defined.
-        Next Obligation. t. Defined.
-        Next Obligation. t. Defined.
-        Next Obligation. t. Defined.
-        Next Obligation. t. Defined.
-        Next Obligation. t. Defined.
-        Next Obligation. t. Defined.
-        Next Obligation. t. Defined.
-        Next Obligation. t. Defined.
-        Next Obligation. t. Defined.
-        Show Profile.
-        Obligations.
-        Next Obligation.
-          repeat t''.
-          subst_body; simpl in *.
-          specialize (X (transitivity (str_le1_append _ _ _) H)).
-          SearchAbout (_ ≤s _).
-          subst_body; simpl.
-
-          do 2 try inversion_one_head_hnf @minimal_parse_of_production.
-
-          repeat t''.
-          change unit.
-          unfold parse_of_production__of__minimal_parse_of_production.
-          hnf.
-          unfold Forall_parse_of_production.
-
-          constructor.
-          unfold parse_of_production__of__minimal_parse_of_production.
-          constructor.
-        Solve Obligation 1 using t.
-        Solve Obligation 2 using t.
-        Solve Obligation 3 using t.
-        Solve Obligation 4 using t.
-        Solve Obligation 5 using t.
-        Solve Obligation 6 using t.
-        Solve Obligation 7 using t.
-        Solve Obligation 8 using t.
-        Solve Obligation 9 using t.
-        Solve Obligation 10 using t.
-        Solve Obligation 11 using t.
-        Solve Obligation 12 using t.
-        Solve Obligation 13 using t.
-        Solve Obligation 14 using t.
-        Solve Obligation 1 using t.
-        Solve Obligation 1 using t.
-        Obligations.
-        Next Obligation.
-          t.
-          repeat t''.
-          Print minimal_parse_of_production.
-          exists (MinParseProductionNil _ _ _ _ _ _ _).
-          exists (MinParseProductionNil _ _ _ _ _ _ _).
-          exfalso.
-          repeat t'.
-          t''.
-          t''.
-          t''.
-          t''.
-          t''.
-          t''.
-          t''.
-          t''.
-
-          repeat t''.
-          t'.
-          exfalso; t.
-
-          SearchAbout (?x =s _).
-
-          t''.
-          t''.
-
-
-          t''.
-          t''.
-          t''.
-          t''.
-          t''.
-          t''.
-          t''.
-          t''.
-
-          exfalso; t.
-        Defined.
-        Next Obligation.
-          t.
-        Defined.
-        Next Obligation.
-          t.
-        Defined.
-        Next Obligation.
-
-          t.
-          repeat t''; t.
-        Defined.
-
-        Next Obligation.
-          t.
-
-          repeat t''.
-          match goal with |- _ * _ => split end.
-          t''.
-          repeat t''.
-
-
-
-          match goal with
-            | [ H : parse_of_item _ _ ?s (Terminal ch) |- _ ] => atomic s; inversion H
-          end.
-          subst x.
-          destruct H2.
-        Defined.
-
-          repeat t''.
-          t.
-          unfold T_nonterminal_name_success in *.
-          t''.
-          t.
-          t''.
-        Defined.
-
-          t'.
-          t'.
-          t'.
-          t'.
-          t'.
-          t'.
-          t'.
-          t'.
-          t'.
-          t'.
-          t'.
-          t'.
-          t'.
-          t'.
-          t'.
-          t'.
-          t'.
-          first [ t''
-                | congruence
-                | omega
-                | match goal with x : _ |- _ => exists (MinParseNonTerminal x) end
-                | match goal with H : (?x =s ?x) = false |- _ => erewrite (proj2 (bool_eq_correct _ _ _)) in H by reflexivity end ].
-          first [ intro
-                | match goal with H : ?A -> ?B, H' : ?A |- _ => specialize (H H') end
-                | progress hnf in *
-                | progress eauto with minimal_instance_db
-                | progress destruct_head @StringWithSplitState
-                | progress destruct_head option
-                | progress destruct_head sigT
-                | progress destruct_head prod
-                | progress simpl in *
-                | progress subst ].
-
-          t'.
-          t'.
-          t'.
-
-          Print minimal_parse_of_item.
-          destruct x.
-          unfold parse_of_item_name__of__minimal_parse_of_name' in f.
-          hnf in f.
-          unfold parse_of_item
-
-          t'.
-
-          simpl in *.
-
-          unfold T_nonterminal_name_success
-          hnf in *.
-
-          eapply H_prod_split'; eauto.
-          Grab Existential Variables.
-          assumption.
-        Defined.
+        Obligation 11. t. Defined.
+        Obligation 12. t. Defined.
+        Obligation 13. t. Defined.
+        Obligation 14. t. Defined.
+        Obligation 15. t. Defined.
       End common.
-
-      Definition minimal_parse_nonterminal_name
-                 (split_list_complete
-                  : forall str0 valid it its str pf,
-                      @split_list_completeT str0 valid valid it its str pf (split_string_for_production it its str))
-      : forall (nonterminal_name : string)
-               (str : StringWithSplitState String (split_stateT (include_nonterminal_name _ nonterminal_name))),
-          sum (T_nonterminal_name_success str initial_nonterminal_names_data nonterminal_name str)
-              (T_nonterminal_name_failure str initial_nonterminal_names_data nonterminal_name str)
-        := @parse_nonterminal_name _ String G (minimal_parser_dependent_types_extra_data split_list_complete).
-    End parts.
-  End minimal.
-End recursive_descent_parser.
-    Section parts.
-      Section common.
-        Section types.
-          Context (str0 : String)
-                  (valid : nonterminal_names_listT).
-
-          Definition T_name_success  (name : string) : Type
-            := minimal_parse_of_name String G initial_names_data is_valid_name remove_name
-                                     str0 valid str name.
-          Definition T_name_failure (name : string) : Type
-            := T_name_success name -> False.
-
-          Definition T_item_success (it : item CharType) : Type
-            := minimal_parse_of_item String G initial_names_data is_valid_name remove_name
-                                     str0 valid str it.
-          Definition T_item_failure (it : item CharType) : Type
-            := T_item_success it -> False.
-
-          Definition T_production_success (prod : production CharType) : Type
-            := minimal_parse_of_production String G initial_names_data is_valid_name remove_name
-                                           str0 valid str prod.
-
-          Definition T_production_failure (prod : production CharType) : Type
-            := T_production_success prod -> False.
-
-          Definition T_productions_success (prods : productions CharType) : Type
-            := minimal_parse_of String G initial_names_data is_valid_name remove_name
-                                str0 valid str prods.
-
-          Definition T_productions_failure (prods : productions CharType) : Type
-            := T_productions_success prods -> False.
-        End types.
-
-        Global Instance minimal_parser_dependent_types_data
-        : @parser_dependent_types_dataT _ String
-          := {| T_name_success := T_name_success;
-                T_name_failure := T_name_failure;
-                T_item_success := T_item_success;
-                T_item_failure := T_item_failure;
-                T_production_success := T_production_success;
-                T_production_failure := T_production_failure;
-                T_productions_success := T_productions_success;
-                T_productions_failure := T_productions_failure |}.
-
-
-        Definition split_list_completeT
-                   (str0 : StringWithSplitState String split_stateT)
-                   valid1 valid2
-                   (str : StringWithSplitState String split_stateT) (pf : str ≤s str0)
-                   (split_list : list (StringWithSplitState String split_stateT * StringWithSplitState String split_stateT))
-                   (prod : production CharType)
-          := match prod return Type with
-               | nil => True
-               | it::its => ({ s1s2 : StringWithSplitState String split_stateT * StringWithSplitState String split_stateT
-                                      & (fst s1s2 ++ snd s1s2 =s str)
-                                        * (minimal_parse_of_item _ G initial_names_data is_valid_name remove_name str0 valid1 (fst s1s2) it)
-                                        * (minimal_parse_of_production _ G initial_names_data is_valid_name remove_name str0 valid2 (snd s1s2) its) }%type)
-                            -> ({ s1s2 : StringWithSplitState String split_stateT * StringWithSplitState String split_stateT
-                                         & (In s1s2 split_list)
-                                           * (minimal_parse_of_item _ G initial_names_data is_valid_name remove_name str0 valid1 (fst s1s2) it)
-                                           * (minimal_parse_of_production _ G initial_names_data is_valid_name remove_name str0 valid2 (snd s1s2) its) }%type)
-             end.
-
-        Lemma H_prod_split'_helper
-              (str0 : StringWithSplitState String split_stateT)
-              (valid : names_listT)
-              (it : item CharType) (its : list (item CharType))
-              (str strs : StringWithSplitState String split_stateT)
-              (p_it : minimal_parse_of_item String G initial_names_data is_valid_name remove_name str0 valid str it)
-              (p_its : minimal_parse_of_production String G initial_names_data is_valid_name remove_name str0 valid strs its)
-              (ls : list
-                      (StringWithSplitState String split_stateT *
-                       StringWithSplitState String split_stateT))
-              (Hin : In (str, strs) ls)
-              (H : fold_right
-                     Datatypes.prod
-                     unit
-                     (map
-                        (fun s1s2 =>
-                           let s1 := fst s1s2 in
-                           let s2 := snd s1s2 in
-                           ((@T_item_failure str0 s1 valid it * @T_production_failure str0 s2 valid its)
-                            + (@T_item_success str0 s1 valid it * @T_production_failure str0 s2 valid its)
-                            + (@T_item_failure str0 s1 valid it * @T_production_success str0 s2 valid its))%type)
-                        ls))
-        : False.
-        Proof.
-          induction ls; simpl in *; trivial; [].
-          destruct_head or; subst;
-          destruct_head prod; eauto; [].
-          destruct_head sum; destruct_head prod;
-          unfold T_item_failure, T_item_success, T_production_failure, T_production_success in *;
-          eauto.
-        Qed.
-
-        Definition H_prod_split'
-                   (str0 str : StringWithSplitState String split_stateT)
-                   (valid : names_listT)
-                   pf it its
-                   (split_list_complete : @split_list_completeT str0 valid valid str pf (split_string_for_production str (it::its)) (it::its))
-        : @split_string_lift_T _ String _ str0 str valid it its (split_string_for_production str).
-        Proof.
-          clear -split_list_complete.
-          intros H pf' H'; hnf in H', split_list_complete.
-          destruct str as [str st]; simpl in *.
-          inversion H'; clear H'; subst.
-          specialize (fun s1 s2 b
-                      => split_list_complete
-                           (existT _ ({| string_val := s1 ; state_val := st |},
-                                      {| string_val := s2 ; state_val := st |})
-                                   b)); simpl in *.
-          let p_it := hyp_with_head @minimal_parse_of_item in
-          let p_its := hyp_with_head @minimal_parse_of_production in
-          specialize (fun pf => split_list_complete _ _ (pf, p_it, p_its)).
-          repeat match goal with
-                   | [ H : ?T -> ?A |- _ ]
-                     => let H' := fresh in
-                        assert (H' : T) by (apply bool_eq_correct; reflexivity);
-                          specialize (H H'); clear H'
-                   | _ => progress destruct_sig
-                 end.
-          eapply H_prod_split'_helper; eassumption.
-        Qed.
-
-        Definition H_prod_split''
-                   (str0 str : StringWithSplitState String split_stateT)
-                   (valid : names_listT)
-                   prod
-                   (split_list_complete : forall pf, @split_list_completeT str0 valid valid str pf (split_string_for_production str prod) prod)
-        : match prod return Type with
-            | nil => unit
-            | it::its => @split_string_lift_T _ String _ str0 str valid it its (split_string_for_production str)
-          end.
-        Proof.
-          unfold split_string_lift_T.
-          destruct prod.
-          { constructor. }
-          { intro pf. apply H_prod_split' with (pf := pf); try apply split_list_complete; assumption. }
-        Defined.
-
-        Hint Constructors minimal_parse_of minimal_parse_of_name minimal_parse_of_production minimal_parse_of_item unit : minimal_instance_db.
-
-        Local Ltac t'' :=
-          first [ intro
-                | progress hnf in *
-                | progress eauto with minimal_instance_db
-                | progress destruct_head @StringWithSplitState
-                | progress simpl in *
-                | progress subst
-                | match goal with H : (_ =s _) = true |- _ => apply bool_eq_correct in H end ].
-
-        Local Ltac t' :=
-          first [ t''
-                | congruence
-                | omega
-                | match goal with H : (?x =s ?x) = false |- _ => erewrite (proj2 (bool_eq_correct _ _ _)) in H by reflexivity end ].
-
-        Local Ltac t :=
-          repeat intro;
-          match goal with
-            | [ |- False ]
-              => abstract (
-                     repeat t';
-                     do 2 try inversion_one_head_hnf @minimal_parse_of_name;
-                     repeat t';
-                     do 2 try inversion_one_head_hnf @minimal_parse_of_item;
-                     repeat t';
-                     do 2 try inversion_one_head_hnf @minimal_parse_of_production;
-                     repeat t';
-                     do 2 try inversion_one_head_hnf @minimal_parse_of;
-                     repeat t'
-                   )
-            | _ => try solve [ repeat t'' ]
-          end.
-
-        Local Obligation Tactic := t.
-
-        Global Program Instance minimal_parser_dependent_types_extra_data
-                (split_list_complete : forall str0 str valid prod pf, @split_list_completeT str0 valid valid str pf (split_string_for_production str prod) prod)
-        : @parser_dependent_types_extra_dataT _ String G.
-        Next Obligation.
-          hnf; apply H_prod_split''.
-          eauto.
-        Defined.
-      End common.
-
-      Definition minimal_parse_name
-                 (split_list_complete
-                  : forall str0 str valid prod pf,
-                      @split_list_completeT str0 valid valid str pf (split_string_for_production str prod) prod)
-      : forall (str : StringWithSplitState String split_stateT)
-               (name : string),
-          sum (T_name_success str str initial_names_data name)
-              (T_name_failure str str initial_names_data name)
-        := @parse_name _ String G (minimal_parser_dependent_types_extra_data split_list_complete).
     End parts.
   End minimal.
 End recursive_descent_parser.
